src/Parsers/Refinement/Tactics.v
@@ -46,8 +46,31 @@ Ltac start_honing_ri repInv :=
 Ltac start_honing :=
   eapply SharpenStep;
   [ solve [ apply FirstStep ] | ];
-  unfold rindexed_spec, rindexed_spec'; simpl;
-  unfold forall_reachable_productions_if_eq; simpl.
+  unfold rindexed_spec, rindexed_spec';
+  cbv beta iota zeta delta [expanded_fallback_list' BaseTypes.production_carrierT BaseTypes.nonterminals_listT BaseTypes.nonterminal_carrierT RDPList.rdp_list_predata Carriers.default_production_carrierT Carriers.default_nonterminal_carrierT BaseTypes.to_production RDPList.rdp_list_to_production expanded_fallback_list'_body forall_reachable_productions_if_eq];
+  lazymatch goal with
+  | [ |- context[List.fold_right _ _ ?ls] ]
+    => let ls' := (eval lazy in ls) in
+       change ls with ls'
+  end;
+  change @List.length with @BooleanRecognizerOptimized.opt2.opt2.length;
+  change @fst with @BooleanRecognizerOptimized.opt2.opt2.fst at 1 3;
+  change @snd with @BooleanRecognizerOptimized.opt2.opt2.snd at 1 3 4;
+  cbv beta iota zeta delta [to_production_opt fst snd Lookup_idx];
+  simpl @List.map;
+  cbv beta iota zeta delta [List.fold_right List.nth Operations.List.drop has_only_terminals];
+  simpl @List.length;
+  change @BooleanRecognizerOptimized.opt2.opt2.length with @List.length;
+  change @BooleanRecognizerOptimized.opt2.opt2.fst with @fst;
+  change @BooleanRecognizerOptimized.opt2.opt2.snd with @snd;
+  simpl @List.length;
+  repeat match goal with
+         | [ |- appcontext G[FixedLengthLemmas.collapse_length_result ?x] ]
+           => let a := constr:(FixedLengthLemmas.collapse_length_result x) in
+              let a' := (eval lazy in a) in
+              progress change a with a'
+         end;
+  simpl.
 
 Tactic Notation "start" "honing" "parser" "representation" "using" open_constr(repInv)
   := (lazymatch goal with
